theories/tree_borrows/disjoint.v
@@ -1,4 +1,189 @@
-From simuliris.tree_borrows Require Import lang_base notation bor_semantics.
+From simuliris.tree_borrows Require Import lang_base notation bor_semantics tree tree_lemmas.
+
+Lemma insert_eqv_rel t t' (ins:item) (tr:tree item) (search:Tprop item)
+  {search_dec:forall it, Decision (search it)} :
+  ~IsTag t ins ->
+  ~IsTag t' ins ->
+  StrictParentChildIn t t' tr <-> StrictParentChildIn t t' (insert_child_at tr ins search).
+Proof.
+  intros Nott Nott'; unfold ParentChildIn.
+  induction tr; simpl; auto.
+  destruct (decide (search data)).
+  + rewrite IHtr1; clear IHtr1. rewrite IHtr2; clear IHtr2.
+    simpl.
+    split; intro Hyp.
+    - destruct Hyp as [Hyp0 [Hyp1 Hyp2]].
+      try repeat split; auto.
+intro H; right; left. eapply insert_preserves_exists; auto.
+    - destruct Hyp as [Hyp0 [Hyp1 [Hyp21 [Hyp22 _]]]].
+      try repeat split; auto.
+      intro H; destruct (Hyp0 H) as [|[|]]; [contradiction| |contradiction].
+      eapply insert_false_infer_exists; eauto.
+  + rewrite IHtr1; clear IHtr1. rewrite IHtr2; clear IHtr2.
+    simpl.
+split; intro Hyp.
+    - destruct Hyp as [Hyp0 [Hyp1 Hyp2]].
+      try repeat split; auto.
+      intro H; auto.
+      apply insert_preserves_exists; auto.
+    - destruct Hyp as [Hyp0 [Hyp1 Hyp2]].
+      try repeat split; auto.
+      intro H; auto.
+      eapply insert_false_infer_exists; eauto.
+Qed.
+
+Lemma insert_produces_StrictParentChild t (ins:item) (tr:tree item) :
+  ~IsTag t ins ->
+  StrictParentChildIn t ins.(itag) (insert_child_at tr ins (IsTag t)).
+Proof.
+  intro Nott.
+  unfold StrictParentChildIn.
+  induction tr; simpl; auto.
+  destruct (decide (IsTag t data)) eqn:Found; simpl.
+  - try repeat split; auto.
+    intro H; left; easy.
+  - try repeat split; auto.
+    intro H; contradiction.
+Qed.
+
+Lemma StrictParentChild_transitive t t' t'' (tr:tree item) :
+  StrictParentChildIn t t' tr ->
+  StrictParentChildIn t' t'' tr ->
+  StrictParentChildIn t t'' tr.
+Proof.
+  rewrite /StrictParentChildIn /HasStrictChildTag.
+  induction tr; simpl; auto.
+  intros [Condtt' [Reltt'1 Reltt'2]] [Condt't'' [Relt't''1 Relt't''2]].
+  split; auto.
+  intro H.
+  clear Relt't''1 Reltt'1 IHtr1 IHtr2.
+  pose proof (Condtt' H) as Ex'.
+  clear Condtt' H Condt't'' Reltt'2.
+  (* End of step 1: we have found a t'. Now look for a t''. *)
+  induction tr2; [destruct Ex'|].
+  destruct Relt't''2 as [IfHere [IfLeft IfRight]].
+  destruct Ex' as [Here | [Left | Right]].
+  - simpl in *; right; right; auto.
+  - right; left; auto.
+  - right; right; auto.
+Qed.
+
+Lemma ParentChild_transitive t t' t'' (tr:tree item) :
+  ParentChildIn t t' tr ->
+  ParentChildIn t' t'' tr ->
+  ParentChildIn t t'' tr.
+Proof.
+  unfold ParentChildIn.
+  destruct (decide (t = t')); [subst; tauto|].
+  destruct (decide (t' = t'')); [subst; tauto|].
+  intros Ptt' Pt't''.
+  destruct Ptt'; [contradiction|].
+  destruct Pt't''; [contradiction|].
+  right.
+  eapply StrictParentChild_transitive; eauto.
+Qed.
+
+Lemma insert_produces_StrictParentChild_transitive t t' (ins:item) (tr:tree item) :
+  ~IsTag t ins ->
+  ~IsTag t' ins ->
+  StrictParentChildIn t t' tr ->
+  StrictParentChildIn t ins.(itag) (insert_child_at tr ins (IsTag t')).
+Proof.
+  intros Nott Nott' Ptt'.
+  apply (StrictParentChild_transitive t t' ins.(itag)).
+  - apply insert_eqv_rel; auto.
+  - apply insert_produces_StrictParentChild; auto.
+Qed.
+
+
+Lemma insert_produces_minimal_ParentChild (t t':tag) (ins:item) (tr:tree item) :
+  ~IsTag t ins ->
+  ~IsTag t' ins ->
+  ~t = t' ->
+  ~tree_contains ins.(itag) tr ->
+  StrictParentChildIn t ins.(itag) (insert_child_at tr ins (IsTag t')) ->
+  StrictParentChildIn t t' tr.
+Proof.
+  intros Nott Nott' Diff Absent Pins.
+  unfold tree_contains in Absent.
+  rewrite <- every_not_eqv_not_exists in Absent.
+  induction tr; simpl; auto.
+  simpl in Pins; destruct (decide (IsTag t' data)) as [Tg'|].
+  all: destruct Absent as [Absent0 [Absent1 Absent2]].
+  all: destruct Pins as [Pins0 [Pins1 Pins2]].
+  all: try repeat split.
+  - intro Contra; exfalso; unfold IsTag in Tg'; unfold IsTag in Contra.
+    subst; contradiction.
+  - apply IHtr1; assumption.
+  - apply IHtr2; [|destruct Pins2 as [?[??]]]; assumption.
+  - intro Tg. simpl in Pins0.
+    eapply exists_insert_requires_parent.
+    + exact Absent2.
+    + apply Pins0. exact Tg.
+  - apply IHtr1; assumption.
+  - apply IHtr2; assumption.
+Qed.
+
+Lemma inserted_empty_children (t:tag) (ins:item) (tr:tree item) :
+  ~tree_contains ins.(itag) tr ->
+  every_subtree (fun br => HasRootTag ins.(itag) br -> empty_children br) (insert_child_at tr ins (IsTag t)).
+Proof.
+  move=> Fresh.
+  unfold tree_contains in Fresh.
+  rewrite <- every_not_eqv_not_exists in Fresh.
+  induction tr; simpl; auto.
+  destruct (decide (IsTag t data)); simpl in *.
+  all: destruct Fresh as [Fresh0 [Fresh1 Fresh2]].
+  + try repeat split.
+    - intro; contradiction.
+    - apply IHtr1; exact Fresh1.
+    - apply IHtr2; exact Fresh2.
+  + try repeat split.
+    - intro; contradiction.
+    - apply IHtr1; exact Fresh1.
+    - apply IHtr2; exact Fresh2.
+Qed.
+
+Lemma inserted_not_parent (t:tag) (ins:item) (tr:tree item) :
+  tree_contains t tr ->
+  ~tree_contains ins.(itag) tr ->
+  forall t',
+  tree_contains t' tr ->
+  ~StrictParentChildIn ins.(itag) t' (insert_child_at tr ins (IsTag t)).
+Proof.
+  move=> ContainsParent Fresh t' ContainsOther Rel.
+  assert (~t = ins.(itag)) as Net by (intro; subst; contradiction).
+  assert (~t' = ins.(itag)) as Net' by (intro; subst; contradiction).
+  unfold ParentChildIn in Rel.
+  pose proof (inserted_empty_children t ins tr Fresh) as Contra.
+  clear Fresh.
+  clear ContainsOther.
+  induction tr; simpl in *; try contradiction.
+  destruct (decide (IsTag t data)).
+  all: destruct ContainsParent as [Parent0 | [Parent1 | Parent2]].
+  - simpl in Rel.
+    destruct Rel as [_ [_ [Bad _]]]; apply Net'.
+    unfold IsTag in Bad; destruct Bad; reflexivity.
+  - apply IHtr1.
+    * auto.
+    * destruct Rel as [Rel0 [Rel1 Rel2]]; auto.
+    * destruct Contra as [Contra0 [Contra1 Contra2]]; auto.
+  - apply IHtr2.
+    * auto.
+    * destruct Rel as [Rel0 [Rel1 [Rel20 [Rel21 Rel22]]]]; auto.
+    * destruct Contra as [Contra0 [Contra1 [Contra20 [Contra21 Contra22]]]]; auto.
+  - contradiction.
+  - apply IHtr1.
+    * auto.
+    * destruct Rel as [Rel0 [Rel1 Rel2]]; auto.
+    * destruct Contra as [Contra0 [Contra1 Contra2]]; auto.
+  - apply IHtr2.
+    * auto.
+    * destruct Rel as [Rel0 [Rel1 Rel2]]; auto.
+    * destruct Contra as [Contra0 [Contra1 Contra2]]; auto.
+Qed.
+
+
 
 Lemma create_child_isSome tr tgp tgc :
   forall cids range tr' newp,
@@ -14,29 +199,29 @@ Proof.
   auto.
 Qed.
 
-Lemma item_apply_access_preserves_tag it :
-  forall kind cids rel range it',
+Lemma item_apply_access_preserves_tag kind it :
+  forall cids rel range it',
   item_apply_access kind cids rel range it = Some it' ->
   itag it = itag it'.
 Proof.
-  move=> ???? it'.
+  move=> ??? it'.
   unfold item_apply_access.
-  destruct (permissions_foreach _); simpl; [|intro H; inversion H].
+  destruct (permissions_foreach); simpl; [|intro H; inversion H].
   intro H; injection H; intros; subst.
   simpl; reflexivity.
 Qed.
 
-Lemma join_project_Exists {X} tr prop :
+Lemma join_project_exists {X} tr prop :
   forall tr',
-  tree_join tr = Some tr' ->
-  tree_Exists prop tr' <-> tree_Exists (fun x => exists (v:X), x = Some v /\ prop v) tr.
+  join_nodes tr = Some tr' ->
+  exists_node prop tr' <-> exists_node (fun x => exists (v:X), x = Some v /\ prop v) tr.
 Proof.
   induction tr; intros tr' JoinSome.
   - simpl in JoinSome; injection JoinSome; intros; subst; tauto.
   - simpl in JoinSome.
     destruct data; simpl in *; [|inversion JoinSome].
-    destruct (tree_join tr1); simpl in *; [|inversion JoinSome].
-    destruct (tree_join tr2); simpl in *; [|inversion JoinSome].
+    destruct (join_nodes tr1); simpl in *; [|inversion JoinSome].
+    destruct (join_nodes tr2); simpl in *; [|inversion JoinSome].
     injection JoinSome; intros; subst.
     simpl.
     split; intro H; destruct H as [H0 | [H1 | H2]].
@@ -48,10 +233,10 @@ Proof.
     * right; right. rewrite IHtr2; auto.
 Qed.
 
-Lemma tree_Exists_increasing {X} (prop prop':Tprop X) tr :
-  tree_Exists prop tr ->
-  tree_Forall (fun x => prop x -> prop' x) tr ->
-  tree_Exists prop' tr.
+Lemma exists_node_increasing {X} (prop prop':Tprop X) tr :
+  exists_node prop tr ->
+  every_node (fun x => prop x -> prop' x) tr ->
+  exists_node prop' tr.
 Proof.
   induction tr; simpl; [tauto|].
   intros H Impl; destruct Impl as [Impl0 [Impl1 Impl2]]; destruct H as [H0 | [H1 | H2]].
@@ -60,12 +245,12 @@ Proof.
   - right; right; apply IHtr2; auto.
 Qed.
 
-Lemma tree_Forall_increasing {X} (prop prop':Tprop X) tr :
-  tree_Forall prop tr ->
-  tree_Forall (fun x => prop x -> prop' x) tr ->
-  tree_Forall prop' tr.
+Lemma every_node_increasing {X} (prop prop':Tprop X) tr :
+  every_node prop tr ->
+  every_node (fun x => prop x -> prop' x) tr ->
+  every_node prop' tr.
 Proof.
-  repeat rewrite tree_Forall_forall.
+  repeat rewrite every_node_eqv_universal.
   intros Pre Trans x Ex.
   apply Trans; [exact Ex|].
   apply Pre.
@@ -73,34 +258,42 @@ Proof.
 Qed.
 
 Lemma access_preserves_tags tr tg :
-  forall tr' app cids range dyn_rel,
-  (forall it it' cids rel range, app cids rel range it = Some it' -> itag it = itag it') ->
-  tree_contains tg tr ->
-  tree_apply_access app cids tg range tr dyn_rel = Some tr' ->
-  tree_contains tg tr'.
+  forall tr' tg' app cids range dyn_rel,
+  (forall it cids rel range it', app cids rel range it = Some it' -> itag it = itag it') ->
+  tree_apply_access app cids tg' range tr dyn_rel = Some tr' ->
+  tree_contains tg tr <-> tree_contains tg tr'.
 Proof.
-  move=> tr' app ??? Preserve Contains Access.
+  move=> tr' tg' app ??? Preserve Access.
   unfold tree_apply_access in Access.
   unfold tree_contains in *.
-  rewrite join_project_Exists.
+  rewrite (join_project_exists _ _ tr').
   2: exact Access.
-  rewrite tree_Exists_map.
+  rewrite exists_node_map.
   unfold compose.
-  pose proof (proj1 (join_success_condition (tree_map _ tr)) (mk_is_Some _ _ Access)).
-  rewrite tree_Forall_map in H.
-  eapply tree_Exists_increasing.
-  - exact Contains.
-  - unfold compose in H.
-    rewrite tree_Forall_forall.
-    rewrite tree_Forall_forall in H.
-    intros x Exists Tagx.
-    pose proof (H x Exists) as Hspec.
-    destruct Hspec as [v App].
-    exists v.
-    split; auto.
-    unfold IsTag in *; subst.
-    symmetry.
-    apply (Preserve _ _ _ _ _ App).
+  pose proof (proj1 (join_success_condition (map_nodes _ tr)) (mk_is_Some _ _ Access)).
+  rewrite every_node_map in H.
+  split; intro Contains.
+  * eapply exists_node_increasing.
+    - exact Contains.
+    - unfold compose in H.
+      rewrite every_node_eqv_universal.
+      rewrite every_node_eqv_universal in H.
+      intros x Exists Tagx.
+      pose proof (H x Exists) as Hspec.
+      destruct Hspec as [v App].
+      exists v.
+      split; auto.
+      unfold IsTag in *; subst.
+      symmetry.
+      apply (Preserve _ _ _ _ _ App).
+  * eapply exists_node_increasing.
+    - exact Contains.
+    - rewrite every_node_eqv_universal.
+      intros x Exists xspec.
+      destruct xspec as [v App].
+      destruct App.
+      unfold IsTag in *; subst.
+      apply (Preserve _ _ _ _ _ H0).
 Qed.
 
 Lemma new_item_has_tag tg :
@@ -122,23 +315,68 @@ Proof.
   unfold tree_contains in *.
   destruct (create_child_isSome tr tgp tgc _ _ _ _ CreateChild) as [tr'' [Read Insert]].
   rewrite Insert.
-  apply insert_True_produces_Exists.
+  apply insert_true_produces_exists.
   - apply new_item_has_tag.
-  - eapply (access_preserves_tags _ _ _ _ _ _ _); [|exact ContainsParent|exact Read].
-    intros.
-    eapply item_apply_access_preserves_tag.
-    exact H.
+  - apply (access_preserves_tags _ _ _ _ _ _ _ _ (item_apply_access_preserves_tag _) Read).
+    exact ContainsParent.
 Qed.
 
-(* fresh t -> fresh t' -> insert t -> insert t' -> ~child t t' *)
+Lemma insertion_preserves_tags tr tg :
+  forall tgp tgc cids range tr' newp,
+  tree_contains tg tr ->
+  create_child cids tgp range tgc newp tr = Some tr' ->
+  tree_contains tg tr'.
+Proof.
+  move=> ???? tr' ? Contains CreateChild.
+  unfold tree_contains in *.
+  destruct (create_child_isSome tr _ _ _ _ _ _ CreateChild) as [tr'' [Read Insert]].
+  rewrite Insert.
+  apply insert_preserves_exists.
+  apply (access_preserves_tags _ _ _ _ _ _ _ _ (item_apply_access_preserves_tag _) Read).
+  exact Contains.
+Qed.
+
 Lemma insertion_order_nonchild tr tg tg' :
   tree_contains tg' tr ->
   ~tree_contains tg tr ->
   forall tgp cids range newp tr',
+  tree_contains tgp tr ->
   create_child cids tgp range tg newp tr = Some tr' ->
-  ~ParentChildIn tg tg' tr.
+  ~StrictParentChildIn tg tg' tr'.
 Proof.
-  intros Present Fresh.
+  move=> Present Fresh tgp ??? tr' ParentPresent Insert Contra.
+  unfold create_child in Insert.
+  remember (memory_read _ _ _ _) as tr''.
+  destruct tr'' as [tr''|]; simpl in *; try (inversion Insert; done).
+  injection Insert; intros; subst; clear Insert.
+  symmetry in Heqtr''.
+  assert (tree_contains tg' tr'') as Present'. {
+    erewrite <- access_preserves_tags.
+    - apply Present.
+    - apply item_apply_access_preserves_tag.
+    - exact Heqtr''.
+  } clear Present.
+  assert (~tree_contains tg tr'') as Fresh'. {
+    intro Invert; apply Fresh; erewrite access_preserves_tags.
+    - apply Invert.
+    - apply item_apply_access_preserves_tag.
+    - exact Heqtr''.
+  } clear Fresh.
+  assert (tree_contains tgp tr'') as ParentPresent'. {
+    erewrite <- access_preserves_tags.
+    - apply ParentPresent.
+    - apply item_apply_access_preserves_tag.
+    - exact Heqtr''.
+  } clear ParentPresent.
+  eapply inserted_not_parent with (ins := (create_new_item tg _ _)).
+  - apply ParentPresent'.
+  - simpl; apply Fresh'.
+  - apply Present'.
+  - apply Contra.
+Qed.
+
+
+
 
 
 
