theories/tree_borrows/tree.v
@@ -1,0 +1,114 @@
+From iris.prelude Require Import prelude options.
+
+Implicit Type (V W X Y:Type).
+
+Definition app X : Type := X -> option X.
+Definition Tprop X : Type := X -> Prop.
+
+(** General Preliminaries *)
+
+Definition unwrap {X} (default:X)
+  : option X -> X :=
+  fun o => match o with
+  | Some t => t
+  | None => default
+  end.
+
+Definition option_bind {X Y} (fn:X -> option Y)
+  : option X -> option Y :=
+  fun ox => x ← ox; fn x.
+
+Definition option_join {X}
+  : option (option X) -> option X :=
+  fun oox => ox ← oox; ox.
+
+(* Generic tree
+   Note: we are using the "tilted" representation of n-ary trees
+         where the binary children are the next n-ary sibling and
+         the first n-ary child.
+         This is motivated by the much nicer induction principles
+         we get, but requires more careful definition of the
+         parent-child relationship.
+   *)
+Inductive tree X :=
+  | empty
+  | branch (data:X) (sibling child:tree X)
+  .
+
+Arguments empty {X}.
+Arguments branch {X} data sibling child.
+Definition tbranch X : Type := X * tree X * tree X.
+
+Definition of_branch {X} (br:tbranch X)
+  : tree X :=
+  let '(root, lt, rt) := br in branch root lt rt.
+
+Definition fold_subtrees {X Y} (unit:Y) (combine:tbranch X -> Y -> Y -> Y)
+  : tree X -> Y := fix aux tr : Y :=
+  match tr with
+  | empty => unit
+  | branch data sibling child => combine (data, sibling, child) (aux sibling) (aux child)
+  end.
+
+Definition root {X} (br:tbranch X)
+  : X := let '(r, _, _) := br in r.
+
+Definition fold_nodes {X Y} (unit:Y) (combine:X -> Y -> Y -> Y)
+  : tree X -> Y := fold_subtrees unit (fun subtree sibling child => combine (root subtree) sibling child).
+
+Definition map_nodes {X Y} (fn:X -> Y) : tree X -> tree Y := fold_nodes empty (compose branch fn).
+
+Definition join_nodes {X}
+  : tree (option X) -> option (tree X) := fix aux tr {struct tr} : option (tree X) :=
+  match tr with
+  | empty => Some empty
+  | branch data sibling child =>
+    data ← data;
+    sibling ← aux sibling;
+    child ← aux child;
+    Some $ branch data sibling child
+  end.
+
+Definition every_subtree {X} (prop:Tprop (tbranch X)) (tr:tree X)
+  := fold_subtrees True (fun sub lt rt => prop sub /\ lt /\ rt) tr.
+Global Instance every_subtree_dec {X} prop (tr:tree X) : (forall x, Decision (prop x)) -> Decision (every_subtree prop tr).
+Proof. intro. induction tr; solve_decision. Qed.
+
+Definition exists_subtree {X} (prop:Tprop (tbranch X)) (tr:tree X)
+  := fold_subtrees False (fun sub lt rt => prop sub \/ lt \/ rt) tr.
+Global Instance exists_subtree_dec {X} prop (tr:tree X) : (forall x, Decision (prop x)) -> Decision (exists_subtree prop tr).
+Proof. intro. induction tr; solve_decision. Qed.
+
+Definition every_node {X} (prop:Tprop X) (tr:tree X) := fold_nodes True (fun data lt rt => prop data /\ lt /\ rt) tr.
+Global Instance every_node_dec {X} prop (tr:tree X) : (forall x, Decision (prop x)) -> Decision (every_node prop tr).
+Proof. intro. induction tr; solve_decision. Qed.
+
+Definition exists_node {X} (prop:Tprop X) (tr:tree X) := fold_nodes False (fun data lt rt => prop data \/ lt \/ rt) tr.
+Global Instance exists_node_dec {X} prop (tr:tree X) : (forall x, Decision (prop x)) -> Decision (exists_node prop tr).
+Proof. intro. induction tr; solve_decision. Qed.
+
+Definition exists_strict_child {X} (prop:Tprop X)
+  : Tprop (tbranch X) := fun '(_, _, child) => exists_node prop child.
+Global Instance exists_strict_child_dec {X} prop (tr:tbranch X) :
+  (forall u, Decision (prop u)) -> Decision (exists_strict_child prop tr).
+Proof. intro. solve_decision. Qed.
+
+Definition empty_children {X} (tr:tbranch X)
+  : Prop :=
+  let '(_, _, children) := tr in
+  children = empty.
+
+Definition insert_child_at {X} (tr:tree X) (ins:X) (search:Tprop X) {search_dec:forall x, Decision (search x)} : tree X :=
+  (fix aux tr : tree X :=
+    match tr with
+    | empty => empty
+    | branch data sibling child =>
+      let sibling := aux sibling in
+      let child := aux child in
+      if decide (search data)
+      then branch data sibling (branch ins child empty)
+      else branch data sibling child
+    end
+  ) tr.
+
+
