theories/tree_borrows/tree_lemmas.v
@@ -1,0 +1,402 @@
+From Equations Require Import Equations.
+From iris.prelude Require Import prelude options.
+From stdpp Require Export gmap.
+From simuliris.tree_borrows Require Export lang_base notation tree.
+From iris.prelude Require Import options.
+
+Implicit Type (V W X Y:Type).
+
+Lemma option_map_compose {X Y Z} (fn:X -> Y) (fn':Y -> Z) :
+  forall ox, option_map fn' (option_map fn ox) = option_map (compose fn' fn) ox.
+Proof. intro ox. destruct ox; simpl; auto. Qed.
+
+Lemma option_bind_map_join {X Y} (fn:X -> option Y) :
+  option_bind fn = compose option_join (option_map fn).
+Proof. apply functional_extensionality. intro ox. destruct ox; simpl; auto. Qed.
+
+Lemma join_join_nodes {X} :
+  forall (tr:tree (option (option X))),
+  option_bind join_nodes (join_nodes tr) = join_nodes (map_nodes option_join tr).
+Proof.
+  induction tr; simpl; auto.
+  rewrite <- IHtr1; rewrite <- IHtr2.
+  destruct data; simpl; auto.
+  destruct o; simpl; auto.
+  all: destruct (join_nodes tr1); simpl; auto.
+  all: destruct (join_nodes tr2); simpl; auto.
+  destruct (join_nodes t); simpl; auto.
+Qed.
+
+Lemma join_nodes_omap_comm {X Y} (fn:X -> Y) :
+  forall (tr:tree (option X)),
+  join_nodes (map_nodes (option_map fn) tr) = option_map (map_nodes fn) (join_nodes tr).
+Proof.
+  induction tr; simpl; auto.
+  rewrite IHtr1; rewrite IHtr2; simpl.
+  destruct data; simpl; auto.
+  destruct (join_nodes tr1); simpl; auto.
+  destruct (join_nodes tr2); simpl; auto.
+Qed.
+
+Lemma map_nodes_compose {W X Y} (fn:W -> X) (fn':X -> Y) :
+  forall (tr:tree W),
+  map_nodes fn' (map_nodes fn tr) = map_nodes (compose fn' fn) tr.
+Proof.
+  induction tr; simpl; auto.
+  rewrite IHtr1. rewrite IHtr2; reflexivity.
+Qed.
+
+Lemma join_nodes_delay {X Y} (fn:X -> option Y) :
+  forall (tr:tree (option X)),
+  join_nodes (map_nodes (option_bind fn) tr) = option_bind (compose join_nodes (map_nodes fn)) (join_nodes tr).
+Proof.
+  intro tr.
+  rewrite option_bind_map_join.
+  rewrite option_bind_map_join.
+  rewrite <- map_nodes_compose.
+  rewrite <- join_join_nodes.
+  rewrite join_nodes_omap_comm.
+  rewrite option_bind_map_join.
+  unfold compose.
+  rewrite option_map_compose.
+  f_equal.
+Qed.
+
+Lemma join_success_condition {X} (tr:tree (option X)) :
+  is_Some (join_nodes tr) <-> every_node is_Some tr.
+Proof.
+  induction tr; simpl; split; auto.
+  - intro Computation.
+    destruct data; destruct (join_nodes tr1); destruct (join_nodes tr2).
+    all: simpl in Computation; inversion Computation; inversion H.
+    rewrite <- IHtr1.
+    rewrite <- IHtr2.
+    split; [|split]. all: auto.
+  - intro AllSuccess.
+    destruct AllSuccess as [DataSome [Success1 Success2]].
+    destruct DataSome; rewrite H; clear H; simpl.
+    destruct (proj2 IHtr1 Success1); rewrite H; clear H; simpl.
+    destruct (proj2 IHtr2 Success2); rewrite H; clear H; simpl.
+    auto.
+Qed.
+
+Lemma every_subtree_eqv_universal {X} prop tr :
+  every_subtree prop tr <-> (forall (br:tbranch X), exists_subtree ((=) br) tr -> prop br).
+Proof.
+  induction tr; simpl; [split; [intros; contradiction|tauto]|].
+  rewrite IHtr1. rewrite IHtr2.
+  split; intro Hyp; try repeat split.
+  - destruct Hyp as [Hyp0 [Hyp1 Hyp2]].
+    intros br Eq.
+    destruct Eq as [Eq0 | [Eq1 | Eq2]]; subst; auto.
+  - apply Hyp; left; auto.
+  - intros br Eq; apply Hyp; right; left; assumption.
+  - intros br Eq; apply Hyp; right; right; assumption.
+Qed.
+
+Lemma exists_subtree_eqv_existential {X} prop tr :
+  exists_subtree prop tr <-> (exists (br:tbranch X), exists_subtree ((=) br) tr /\ prop br).
+Proof.
+  induction tr; simpl; [split; [tauto|intro Hyp; destruct Hyp as [_ [Contra _]]; tauto]|].
+  rewrite IHtr1. rewrite IHtr2.
+  split; intro Hyp.
+  - destruct Hyp as [Hyp0 | [Hyp1 | Hyp2]].
+    * eexists; auto.
+    * destruct Hyp1 as [x [Ex Px]].
+      exists x; auto.
+    * destruct Hyp2 as [x [Ex Px]].
+      exists x; auto.
+  - destruct Hyp as [x [[Hyp0 | [Hyp1 | Hyp2]] Px]].
+    * left; subst; auto.
+    * right; left; exists x; auto.
+    * right; right; exists x; auto.
+Qed.
+
+Lemma exists_node_iff_exists_root {X} prop (tr:tree X) :
+  exists_node prop tr <-> exists_subtree (compose prop root) tr.
+Proof. induction tr; simpl; auto. Qed.
+
+Lemma every_node_iff_every_root {X} prop (tr:tree X) :
+  every_node prop tr <-> every_subtree (compose prop root) tr.
+Proof. induction tr; simpl; auto. Qed.
+
+(* NOTE: Yes, the proof is identical to that of every_subtree_eqv_universal,
+   but it does not seem to be provable from it. Indeed the precondition
+   `exists_node ((=) n) tr` is *much weaker* than `exists_subtree ((=) br) tr` *)
+Lemma every_node_eqv_universal {X} prop tr :
+  every_node prop tr <-> (forall (n:X), exists_node ((=) n) tr -> prop n).
+Proof.
+  induction tr; simpl; [split; [intros; contradiction|tauto]|].
+  rewrite IHtr1. rewrite IHtr2.
+  split; intro Hyp; try repeat split.
+  - destruct Hyp as [Hyp0 [Hyp1 Hyp2]].
+    intros br Eq.
+    destruct Eq as [Eq0 | [Eq1 | Eq2]]; subst; auto.
+  - apply Hyp; left; auto.
+  - intros br Eq; apply Hyp; right; left; assumption.
+  - intros br Eq; apply Hyp; right; right; assumption.
+Qed.
+
+Lemma exists_node_eqv_existential {X} prop tr :
+  exists_node prop tr <-> (exists (n:X), exists_node ((=) n) tr /\ prop n).
+Proof.
+  induction tr; simpl; [split; [tauto|intro Hyp; destruct Hyp as [_ [Contra _]]; tauto]|].
+  rewrite IHtr1. rewrite IHtr2.
+  split; intro Hyp.
+  - destruct Hyp as [Hyp0 | [Hyp1 | Hyp2]].
+    * eexists; auto.
+    * destruct Hyp1 as [x [Ex Px]].
+      exists x; auto.
+    * destruct Hyp2 as [x [Ex Px]].
+      exists x; auto.
+  - destruct Hyp as [x [[Hyp0 | [Hyp1 | Hyp2]] Px]].
+    * left; subst; auto.
+    * right; left; exists x; auto.
+    * right; right; exists x; auto.
+Qed.
+
+Lemma tree_permute_fold_map {X Y Z} (tr:tree X) (unit:Z) (combine:Y -> Z -> Z -> Z) (fn:X -> Y) :
+  fold_nodes unit combine (map_nodes fn tr) = fold_nodes unit (fun data lt rt => combine (fn data) lt rt) tr.
+Proof.
+  induction tr; simpl; auto.
+  rewrite IHtr1. rewrite IHtr2.
+  reflexivity.
+Qed.
+
+Lemma every_node_map {X Y} (tr:tree X) (fn:X -> Y) (prop:Y -> Prop) :
+  every_node prop (map_nodes fn tr) <-> every_node (compose prop fn) tr.
+Proof.
+  unfold every_node.
+  rewrite tree_permute_fold_map.
+  tauto.
+Qed.
+
+Lemma exists_node_map {X Y} (tr:tree X) (fn:X -> Y) (prop:Y -> Prop) :
+  exists_node prop (map_nodes fn tr) <-> exists_node (compose prop fn) tr.
+Proof.
+  unfold exists_node.
+  rewrite tree_permute_fold_map.
+  tauto.
+Qed.
+
+Lemma every_not_eqv_not_exists {X} (prop:Tprop X) (tr:tree X) :
+  every_node (compose not prop) tr
+  <-> ~exists_node prop tr.
+Proof.
+  unfold every_node.
+  split.
+  - intros All Exists.
+    induction tr; simpl; auto.
+    inversion Exists as [Ex0 | [Ex1 | Ex2]]; simpl.
+    all: inversion All as [All0 [All1 All2]]; auto.
+  - intros nExists.
+    induction tr; simpl; auto.
+    try repeat split.
+    (* Now swap the goal and the hypothesis that are all negated *)
+    all: try apply IHtr1.
+    all: try apply IHtr2.
+    all: intro; apply nExists.
+    all: simpl; auto.
+Qed.
+
+(*
+Lemma exists_child_transitive {X} (search search':Tprop X) :
+  forall tr,
+  exists_node search tr ->
+  tree_AtNode search (tree_ChildExists search') tr ->
+  exists_node search' tr.
+Proof.
+  intros tr Exists Search.
+  induction tr; simpl; auto.
+  destruct Search as [Search0 [Search1 Search2]].
+  destruct Exists as [Exists0 | [Exists1 | Exists2]]; auto.
+  destruct (Search0 Exists0); auto.
+Qed.
+
+Lemma AtNodeExists_transitive {X} (search search' search'':Tprop X) :
+  forall tr,
+  tree_AtNode search (tree_ChildExists search') tr ->
+  tree_AtNode search' (tree_ChildExists search'') tr ->
+  tree_AtNode search (tree_ChildExists search'') tr.
+Proof.
+  intros tr Search Search'.
+  induction tr; auto.
+  destruct Search' as [Search' [Search'1 Search'2]].
+  destruct Search as [Search [Search1 Search2]].
+  pose Found1 := (IHtr1 Search1 Search'1).
+  pose Found2 := (IHtr2 Search2 Search'2).
+  simpl; try repeat split; auto.
+  clear Found1; clear Found2; clear IHtr1; clear IHtr2.
+  intro Found; destruct (Search Found) as [Found' | FoundSub].
+  - destruct (Search' Found') as [Found'' | Found'Sub]; auto.
+  - right; clear Found; clear Search; clear Search1; clear Search2.
+    clear Search'.
+    apply (ExistsAtNode_transitive search'); auto.
+Qed.
+*)
+
+Lemma insert_true_preserves_every {X} (tr:tree X) (ins:X) (search prop:Tprop X)
+  {search_dec:forall x, Decision (search x)} :
+  prop ins ->
+  every_node prop tr <-> every_node prop (insert_child_at tr ins search).
+Proof.
+  intro PropIns.
+  induction tr; simpl; auto.
+  destruct (decide (search data)) eqn:Found.
+  (* For most cases, this is straightforward: destruct all and apply inductive hypotheses *)
+  all: split; intro H.
+  all: destruct H as [HData [H1 H2]].
+  all: repeat try split; auto.
+  all: try apply IHtr1; auto.
+  all: try apply IHtr2; auto.
+  (* The one case where this is nontrivial is the case where we did find the object,
+     because IH handles (branch data sibling child) and we need (branch data (insert sibling) child) *)
+  inversion H2 as [HIns [H2' HE]]; auto.
+Qed.
+
+Lemma insert_never_unchanged {X} (tr:tree X) (ins:X) (search prop:Tprop X)
+  {search_dec:forall x, Decision (search x)} :
+  every_node (compose not search) tr ->
+  insert_child_at tr ins search = tr.
+Proof.
+  induction tr; simpl; auto; intro H.
+  destruct H as [H0 [H1 H2]].
+  destruct (decide (search data)); [contradiction|].
+  rewrite (IHtr1 H1).
+  rewrite (IHtr2 H2).
+  reflexivity.
+Qed.
+
+Lemma insert_preserves_exists {X} (ins:X) (tr:tree X) (search prop:Tprop X)
+  {search_dec:forall x, Decision (search x)} :
+  exists_node prop tr -> exists_node prop (insert_child_at tr ins search).
+Proof.
+  intros Exists.
+  induction tr; simpl; auto.
+  destruct (decide (search data)).
+  all: simpl.
+  all: inversion Exists as [Ex0 | [Ex1 | Ex2]].
+  all: auto.
+  right; right; right; left; auto.
+Qed.
+
+Lemma insert_false_infer_exists {X} (ins:X) (tr:tree X) (search prop:Tprop X)
+  {search_dec:forall x, Decision (search x)} :
+  ~prop ins ->
+  exists_node prop (insert_child_at tr ins search) ->
+  exists_node prop tr.
+Proof.
+  intros nIns Exists.
+  induction tr; simpl; auto.
+  simpl in Exists.
+  destruct (decide (search data)).
+  all: inversion Exists as [Ex0 | [Ex1 | Ex2]].
+  all: auto.
+  right; right; auto.
+  inversion Ex2 as [Ex20 | [Ex21 | Ex22]]; auto.
+  - contradiction Ex20.
+  - contradiction Ex22.
+Qed.
+
+Lemma insert_true_produces_exists {X} (ins:X) (tr:tree X) (search prop:Tprop X)
+  {search_dec:forall x, Decision (search x)} :
+  prop ins ->
+  exists_node search tr ->
+  exists_node prop (insert_child_at tr ins search).
+Proof.
+  intros Ins Exists.
+  induction tr; simpl; auto.
+  destruct (decide (search data)).
+  - right; right; left; done.
+  - destruct Exists as [Ex0 | [Ex1 | Ex2]].
+    * contradiction.
+    * right; left; auto.
+    * right; right; auto.
+Qed.
+
+(*
+Lemma insert_preserves_ChildExists {X} (ins:X) (tr:tree X) (search prop:Tprop X)
+  {search_dec:forall x, Decision (search x)} :
+  tree_ChildExists prop tr -> tree_ChildExists prop (insert_child_at tr ins search).
+Proof.
+  intro Exists.
+  destruct tr; simpl; auto.
+  destruct (decide (search data)) eqn:Found; simpl; auto.
+  all: simpl in Exists.
+  all: inversion Exists as [Ex0 | Ex2]; auto.
+  1: right; right; left; apply insert_preserves_Exists; auto.
+  right; apply insert_preserves_Exists; auto.
+Qed.
+*)
+
+Lemma exists_insert_requires_parent {X} (ins:X) (search prop:Tprop X)
+  {search_dec:forall x, Decision (search x)} :
+  forall tr,
+  every_node (compose not prop) tr ->
+  exists_node prop (insert_child_at tr ins search) ->
+  exists_node search tr.
+Proof.
+  induction tr; simpl; auto.
+  intros Hyp Ex.
+  destruct Hyp as [Nprop [Absent1 Absent2]].
+  destruct (decide (search data)) eqn:Found; auto.
+  all: destruct Ex as [Here | [Ex1 | Ex2]]; auto.
+  contradiction.
+Qed.
+
+Lemma remove_false_preserves_exists {X} (ins:X) (search prop:Tprop X)
+  {search_dec:forall x, Decision (search x)} :
+  ~prop ins ->
+  forall tr,
+  exists_node prop (insert_child_at tr ins search) ->
+  exists_node prop tr.
+Proof.
+  intros Nprop tr Hyp; induction tr; simpl in *; auto.
+  destruct (decide (search data)) eqn:Found; auto.
+  all: destruct Hyp as [Here | [Hyp1 | Hyp2]]; auto.
+  right; right. destruct Hyp2 as [Contra | [Hyp2Sub | Hyp2Empty]]; auto; contradiction.
+Qed.
+
+Lemma exists_subtree_transitive br prop (tr:tree item) :
+  exists_subtree (eq br) tr ->
+  exists_subtree prop (of_branch br) ->
+  exists_subtree prop tr.
+Proof.
+  induction tr; auto.
+  intros Sub1 Sub2.
+  destruct Sub1 as [Sub10 | [Sub11 | Sub12]].
+  - destruct br as [[iroot ileft] iright]; simpl in *.
+    injection Sub10; intros; subst; auto.
+  - right; left. apply IHtr1; auto.
+  - right; right. apply IHtr2; auto.
+Qed.
+
+Lemma every_subtree_transitive br prop (tr:tree item) :
+  every_subtree (eq br) tr ->
+  every_subtree prop (of_branch br) ->
+  every_subtree prop tr.
+Proof.
+  induction tr; auto.
+  intros Sub1 Sub2.
+  destruct Sub1 as [Sub10 [Sub11 Sub12]].
+  destruct br as [[iroot ileft] iright].
+  injection Sub10; intros; subst.
+  destruct Sub2 as [Sub20 [Sub21 Sub22]].
+  try repeat split; auto.
+Qed.
+
+Lemma exists_node_transitive br prop (tr:tree item) :
+  exists_subtree (eq br) tr ->
+  exists_node prop (of_branch br) ->
+  exists_node prop tr.
+Proof.
+  repeat rewrite exists_node_iff_exists_root.
+  apply exists_subtree_transitive.
+Qed.
+
+(*
+Lemma strict_child_of_exists_exists br prop (tr:tree item) :
+  exists_subtree (eq br) tr ->
+  exists_strict_child prop br ->
+  exists_node prop tr.
+  *)
